Improve Selectors.Examples

pulse/examples/steel/Selectors.Examples.fst
@@ -1,6 +1,6 @@
 module Selectors.Examples
 
-// open Steel.Effect.Atomic
+open Steel.Effect.Atomic
 open Steel.Effect
 open Steel.Reference
 
@@ -8,19 +8,6 @@ open Steel.Reference
 
 #push-options "--fuel 0 --ifuel 0 --ide_id_info_off"
 
-module T = FStar.Tactics
-
-#set-options "--print_full_names --log_queries"
-
-let debug(r r':ref int) : Steel unit
-  (vptr r `star` vptr r') (fun _ -> vptr r `star` vptr r')
-  (requires fun _ -> True)
-  (ensures fun _ _ h1 -> sel r h1 == 0)
-  by (T.norm normal_steps; T.dump "here")
-  = write r 1;
-    write r 0
-
-(*
 let swap (#a:Type0) (r1 r2:ref a) : Steel unit
   (vptr r1 `star` vptr r2)
   (fun _ -> vptr r1 `star` vptr r2)
@@ -37,11 +24,11 @@ let test0 (r:ref int) : Steel unit
   (vptr r) (fun _ -> vptr r)
   (requires fun h -> sel r h == 0)
   (ensures fun _ _ h1 -> sel r h1 == 1)
-  = let h = get () in
-    assert (sel r h == 0);
+  = let x = gget (vptr r) in
+    assert (x == Ghost.hide 0);
     write r 1;
-    let h1 = get() in
-    assert (sel r h1 == 1);
+    let x = gget (vptr r) in
+    assert (x == Ghost.hide 1);
     write r 1
 
 let test1 (r:ref int) : Steel unit
@@ -58,8 +45,6 @@ let test2 (r1 r2:ref int) : Steel unit
   = write r1 0;
     write r1 0
 
-module T = FStar.Tactics
-
 let test3 (r1 r2 r3:ref int) : Steel unit
   (vptr r1 `star` (vptr r2 `star` vptr r3)) (fun _ -> vptr r1 `star` (vptr r2 `star` vptr r3))
   (requires fun _ -> True)
@@ -68,11 +53,10 @@ let test3 (r1 r2 r3:ref int) : Steel unit
     sel r2 h0 == sel r2 h1 /\
     sel r3 h0 == sel r3 h1
   )
-  by (T.norm normal_steps)
-  = let h0 = get () in
+  = let x2_0 = gget (vptr r2) in
     write r1 1;
-    let h1 = get() in
-    assert (sel r1 h1 == 1);
-    assert (sel r2 h0 == sel r2 h1);
+    let x1_1 = gget (vptr r1) in
+    let x2_1 = gget (vptr r2) in
+    assert (x1_1 == Ghost.hide 1);
+    assert (x2_0 == x2_1);
     write r1 0
-*)
